Arm/Insts/DPI/Logical_imm.lean
@@ -1,0 +1,85 @@
+/-
+Copyright (c) 2023 Amazon.com, Inc. or its affiliates. All Rights Reserved.
+Author(s): Yan Peng
+-/
+-- AND, ORR, EOR, ANDS (immediate): 32- and 64-bit versions
+
+import Arm.Decode
+import Arm.Insts.Common
+
+namespace DPI
+
+open Std.BitVec
+
+def decode_op (opc : BitVec 2) : LogicalImmType :=
+  match opc with
+  | 00#2 => LogicalImmType.AND
+  | 01#2 => LogicalImmType.ORR
+  | 10#2 => LogicalImmType.EOR
+  | 11#2 => LogicalImmType.ANDS
+
+def update_logical_imm_pstate (bv : BitVec n) : PState :=
+  have h: n - 1 - (n - 1) + 1 = 1 := by simp
+  let N := h ▸ (Std.BitVec.extractLsb (n-1) (n-1) bv)
+  let Z := zero_flag_spec bv
+  let C := 0#1
+  let V := 0#1
+  (make_pstate N Z C V)
+
+def exec_logical_imm_op (op : LogicalImmType) (op1 : BitVec n) (op2 : BitVec n)
+  : (BitVec n × Option PState) :=
+  match op with
+  | LogicalImmType.AND => (op1 &&& op2, none)
+  | LogicalImmType.ORR => (op1 ||| op2, none)
+  | LogicalImmType.EOR => (op1 ^^^ op2, none)
+  | LogicalImmType.ANDS =>
+    let result := op1 &&& op2
+    (op1 &&& op2, some (update_logical_imm_pstate result))
+
+@[simp]
+def exec_logical_imm (inst : Logical_imm_cls) (s : ArmState) : ArmState :=
+  if inst.sf = 0#1 ∧ inst.N ≠ 0 then
+    write_err (StateError.Illegal s!"Illegal {inst} encountered!") s
+  else
+    let datasize := 32 <<< inst.sf.toNat
+    let imm := decode_bit_masks inst.N inst.imms inst.immr true datasize
+    match imm with
+    | none => write_err (StateError.Illegal s!"Illegal {inst} encountered!") s
+    | some (imm, _) =>
+      let operand1 := read_gpr datasize inst.Rn s
+      let op := decode_op inst.opc
+      let (result, maybe_pstate) := exec_logical_imm_op op operand1 imm
+      -- State Updates
+      let s'            := write_pc ((read_pc s) + 4#64) s
+      let s'            := match maybe_pstate with
+                           | none => s'
+                           | some pstate => write_pstate pstate s'
+      let s'            := write_gpr datasize inst.Rd result s'
+      s'
+
+----------------------------------------------------------------------
+
+/-- Generate random instructions of the DPI.Logical_imm class. -/
+partial def Logical_imm_cls.rand : IO (Option (BitVec 32)) := do
+  let opc := ← BitVec.rand 2
+  let op  := decode_op opc
+  -- (FIXME) We want to avoid use of SP (i.e., register index
+  -- 31) for AND ORR and EOR since our simulation framework doesn't
+  -- work in such cases.
+  let hi  := if op = LogicalImmType.ANDS then 31 else 30
+  let (inst : Logical_imm_cls) :=
+    { sf    := ← BitVec.rand 1,
+      opc   := opc,
+      N     := ← BitVec.rand 1,
+      immr  := ← BitVec.rand 6,
+      imms  := ← BitVec.rand 6,
+      Rn    := ← BitVec.rand 5 (lo := 0) (hi := hi),
+      Rd    := ← BitVec.rand 5 (lo := 0) (hi := hi)
+    }
+  let datasize := 32 <<< inst.sf.toNat
+  if inst.sf = 0#1 ∧ inst.N = 1#1 ∨ invalid_bit_masks inst.N inst.imms true datasize then
+    Logical_imm_cls.rand
+  else
+    pure (some (inst.toBitVec32))
+
+end DPI
